src/lib/kuiper/Kuiper.Barrier.fsti
@@ -2,6 +2,7 @@ module Kuiper.Barrier
 
 #lang-pulse
 
+open Kuiper.Common
 open Pulse.Lib.Pervasives
 open Pulse.Lib.BigStar
 open FStar.Tactics.V2
@@ -9,25 +10,41 @@ open Kuiper.Base
 open Kuiper.SizeT
 module SZ = FStar.SizeT
 
+(* A barrier over nthreads. This is for specification only,
+there is no runtime representation for, as this models
+the builtin CUDA __syncthreads() function. *)
 [@@erasable]
 val barrier
   (n:nat)
   : Type0
 
+(* A token representing that
+   1) There is a barrier in scope
+   2) We are thread 'tid' in the group
+   3) We are in interation 'it'
+   
+   p and q represent the pre- and postconditions
+   to the barrier_wait for a given thread at a given iteration.
+*)
 val barrier_tok
   (#n:nat)
-  (p : (it:nat -> tid:nat { 0 <= tid /\ tid < n } -> slprop))
-  (q : (it:nat -> tid:nat { 0 <= tid /\ tid < n } -> slprop))
+  (p : (it:nat -> tid:natlt n -> slprop))
+  (q : (it:nat -> tid:natlt n -> slprop))
   (b : barrier n)
   (it : nat)
-  (tid : nat { tid < n })
+  (tid : natlt n)
   : slprop
 
+(* Creating a barrier for n threads. Note how this is a
+   ghost function!. The 'pf' argument is a proof, once and
+   for all, that the resource passing in each barrier_wait is
+   correct, since it shows how all of the p's give all of the 
+   q's at each iteration. *)
 ghost
 fn mk_barrier
   (n: SZ.t { 0 < n /\ n <= max_threads })
-  (p : (it:nat -> tid:nat { 0 <= tid /\ tid < n } -> slprop))
-  (q : (it:nat -> tid:nat { 0 <= tid /\ tid < n } -> slprop))
+  (p : (it:nat -> tid:natlt n -> slprop))
+  (q : (it:nat -> tid:natlt n -> slprop))
   (pf : (it:nat -> stt_ghost unit emp_inames
                   (requires bigstar 0 n (p it))
                   (ensures  fun _ -> bigstar 0 n (q it))))
@@ -35,23 +52,29 @@ fn mk_barrier
   returns  b : erased (barrier n)
   ensures  block_setup n ** bigstar 0 n (barrier_tok p q b 0)
 
-// __syncthreads()
+(* Wait on the barrier. This function blocks until all threads call it
+   simultaneously. Each thread provides the current p
+   and gets the current q. The iteration counter is incremented. *)
 fn barrier_wait
   (#n : erased nat)
-  (#p : (it:nat -> tid:nat { 0 <= tid /\ tid < n } -> slprop))
-  (#q : (it:nat -> tid:nat { 0 <= tid /\ tid < n } -> slprop))
+  (#p : (it:nat -> tid:natlt n -> slprop))
+  (#q : (it:nat -> tid:natlt n -> slprop))
   (b : barrier n)
   (#it : erased nat)
-  (#tid : erased nat { tid < n })
+  (#tid : erased (natlt n))
   requires barrier_tok p q b  it    tid ** p it tid
   ensures  barrier_tok p q b (it+1) tid ** q it tid
 
-ghost
-fn drop_barrier
-  (#n : nat)
-  (#p : (it:nat -> tid:nat { 0 <= tid /\ tid < n } -> slprop))
-  (#q : (it:nat -> tid:nat { 0 <= tid /\ tid < n } -> slprop))
-  (#b : barrier n)
-  (#it: nat)
-  requires bigstar 0 n (barrier_tok p q b it)
-  ensures  emp
+(* I don't think this is really useful, nor even desirable. The API
+should probably enforce we always return a barrier token back, so
+there are never two conflicting specs. So why even have the barrier type...? *)
+
+// ghost
+// fn drop_barrier
+//   (#n : nat)
+//   (#p : (it:nat -> tid:natlt n -> slprop))
+//   (#q : (it:nat -> tid:natlt n -> slprop))
+//   (#b : barrier n)
+//   (#it: nat)
+//   requires bigstar 0 n (barrier_tok p q b it)
+//   ensures  emp
