extraction/ExtractKuiper.fst
@@ -121,7 +121,7 @@ let gpu_translate_expr : translate_expr_t = fun env e ->
 
   (******** BARRIERS ********)
 
-  | MLE_App ({ expr = MLE_Name p } , [u1;u2;u3;u4])
+  | MLE_App ({ expr = MLE_Name p } , [_;u1;u2;u3;u4])
     when string_of_mlpath p = "Kuiper.Barrier.RPM.mbarrier_wait" ->
     EApp (EQualified ([], "__syncthreads"), [ EUnit ])
 
